Added context and data type rules

code/datatypes/cuMin.v
@@ -1,12 +1,42 @@
+Require Import  Datatypes EqNat.
+Local Open Scope nat_scope.
+
+Inductive id : Type :=
+  | Id : nat -> id.
+  
+Definition total_map (A:Type) := id -> A.
+
+Definition partial_map (A:Type) := total_map (option A).
+
+Definition t_empty {A:Type} (v : A) : total_map A :=
+  (fun _ => v).
+  
+
+Definition beq_id id1 id2 :=
+  match id1,id2 with
+    | Id n1, Id n2 => beq_nat n1 n2
+  end.
+  
+Definition t_update {A:Type} (m : total_map A)
+                    (x : id) (v : A) :=
+  fun x' => if beq_id x x' then v else m x'.
+
+Definition empty {A:Type} : partial_map A :=
+  t_empty None.
+
+Definition update {A:Type} (m : partial_map A)
+                  (x : id) (v : A) :=
+  t_update m x (Some v).
+
 Inductive tm : Type :=
-  | tvar : tm
+  | tvar : id -> tm
   | tapp : tm -> tm -> tm
   | tfun : tm -> tm -> tm
   | tlet : tm -> tm -> tm -> tm
   | ttrue : tm
   | tfalse : tm
   | tfailure : tm
-  | tanyting : tm
+  | tanything : tm
   | tzero : tm
   | tsucc : tm -> tm
   | tadd : tm -> tm -> tm
@@ -14,7 +44,7 @@ Inductive tm : Type :=
   | tpair : tm -> tm -> tm
   | tnil : tm
   | tcons : tm -> tm -> tm
-  | tcasep : tm -> tm -> tm (* ? *)
+  | tcasep : tm -> tm -> tm
   | tcaseb : tm -> tm -> tm -> tm
   | tcasel : tm -> tm -> tm -> tm.
   
@@ -25,64 +55,115 @@ Inductive ty : Type :=
   | TList : ty -> ty
   | TPair : ty -> ty -> ty
   | TFun : ty -> ty -> ty.
-  
-Reserved Notation "'|-' t '\in' T" (at level 40).
 
-Inductive has_type : tm -> ty -> Prop :=
-  | T_Var :    |- tvar \in TVar (* ? *)
-  | T_True :   |- ttrue \in TBool
-  | T_False :  |- tfalse \in TBool
-  | T_Zero :   |- tzero \in TNat
-  | T_Succ :   forall e,
-               |- e \in TNat -> 
-               |- (tsucc e) \in TNat
-  | T_Nil :    forall T, |- tnil \in (TList T)
-  | T_App :    forall e1 e2 T1 T2,
-               |- e1 \in (TFun T1 T2) ->
-               |- e2 \in T1 ->
-               |- (tapp e1 e2) \in T2
-  | T_Let :    forall e1 e2 x T1 T2,
-               |- e1 \in T1 ->
-               |- x \in T1 ->
-               |- e2 \in T2 ->
-               |- (tlet x e1 e2) \in T2
+Definition context := partial_map ty.
+
+Reserved Notation "Gamma '|-' T '\in_data'" (at level 40).
+Inductive data : context -> ty -> Prop :=
+  | D_Var :  forall Gamma A, Gamma |- A \in_data (*?*)
+  | D_Bool : forall Gamma, Gamma |- TBool \in_data
+  | D_Nat :  forall Gamma, Gamma |- TNat \in_data
+  | D_List : forall Gamma T,
+               Gamma |- T \in_data ->
+               Gamma |- (TList T) \in_data
+  | D_Pair : forall Gamma T T', 
+               Gamma |- T \in_data ->
+               Gamma |- T' \in_data ->
+               Gamma |- (TPair T T') \in_data
+where "Gamma '|-' T '\in_data'" := (data Gamma T).
+
+Reserved Notation "Gamma '|-' t '\in' T" (at level 40).
+
+Inductive has_type : context -> tm -> ty -> Prop :=
+  | T_Var :    forall Gamma x T,
+               Gamma x = Some T ->
+               Gamma |- tvar x \in T
+  | T_True :   forall Gamma, 
+               Gamma |- ttrue \in TBool
+  | T_False :  forall Gamma,
+               Gamma |- tfalse \in TBool
+  | T_Zero :   forall Gamma,
+               Gamma |- tzero \in TNat
+  | T_Succ :   forall Gamma e,
+               Gamma |- e \in TNat -> 
+               Gamma |- (tsucc e) \in TNat
+  | T_Nil :    forall Gamma T, 
+               Gamma |- tnil \in (TList T)
+  | T_App :    forall Gamma e1 e2 T1 T2,
+               Gamma |- e1 \in (TFun T1 T2) ->
+               Gamma |- e2 \in T1 ->
+               Gamma |- (tapp e1 e2) \in T2
+  | T_Let :    forall Gamma e1 e2 x T1 T2,
+               Gamma |- e1 \in T1 ->
+               Gamma x = Some T1 ->
+               Gamma |- e2 \in T2 ->
+               Gamma |- (tlet (tvar x) e1 e2) \in T2
 (*| T_Fun*)
-  | T_Add :    forall e1 e2,
-               |- e1 \in TNat ->
-               |- e2 \in TNat ->
-               |- (tadd e1 e2) \in TNat
-  | T_EqN :    forall e1 e2,
-               |- e1 \in TNat ->
-               |- e2 \in TNat ->
-               |- (teqn e1 e2) \in TBool
-  | T_Pair:    forall e1 e2 T1 T2,
-               |- e1 \in T1 ->
-               |- e2 \in T2 ->
-               |- (tpair e1 e2) \in (TPair T1 T2)
-  | T_Cons :   forall e1 e2 T,
-               |- e1 \in T ->
-               |- e2 \in (TList T) -> 
-               |- (tcons e1 e2) \in (TList T)
-(*| T_CaseL :  forall e e1 e2 h t T T',
-               |- e \in (TList T') ->
-               |- e1 \in T ->
-               |- h \in T' ->
-               |- t \in (TList T') ->
-               |- e2 \in T1 ->
-               |- (tcasel e e1 e2) \in T
-  | T_CaseP :  forall e e1 T T1 T2
-               |- e \in (TPair T1 T2) ->
-               |- l \in T1 ->
-               |- r \in T2 ->
-               |- e1 \in T ->
-               |- (tcasep e e1) \in T *)
-  | T_CaseB :  forall e e1 e2 T,
-               |- e \in TBool ->
-               |- e1 \in T ->
-               |- e2 \in T ->
-               |- (tcaseb e e1 e2) \in T
-  | T_Fail :   forall T, |- tfailure \in T
+  | T_Add :    forall Gamma e1 e2,
+               Gamma |- e1 \in TNat ->
+               Gamma |- e2 \in TNat ->
+               Gamma |- (tadd e1 e2) \in TNat
+  | T_EqN :    forall Gamma e1 e2,
+               Gamma |- e1 \in TNat ->
+               Gamma |- e2 \in TNat ->
+               Gamma |- (teqn e1 e2) \in TBool
+  | T_Pair:    forall Gamma e1 e2 T1 T2,
+               Gamma |- e1 \in T1 ->
+               Gamma |- e2 \in T2 ->
+               Gamma |- (tpair e1 e2) \in (TPair T1 T2)
+  | T_Cons :   forall Gamma e1 e2 T,
+               Gamma |- e1 \in T ->
+               Gamma |- e2 \in (TList T) -> 
+               Gamma |- (tcons e1 e2) \in (TList T)
+  | T_CaseL :  forall Gamma e e1 e2 h t T T',
+               Gamma h = Some T' ->
+               Gamma t = Some (TList T') ->
+               Gamma |- e \in (TList T') ->
+               Gamma |- e1 \in T ->
+               Gamma |- e2 \in T ->
+               e = (tcons (tvar h) (tvar t)) -> (*?*)
+               Gamma |- (tcasel e e1 e2) \in T
+  | T_CaseP :  forall Gamma e e1 l r T T1 T2,
+               Gamma l = Some T1 ->
+               Gamma r = Some T2 ->
+               Gamma |- e \in (TPair T1 T2) ->
+               e = (tpair (tvar l) (tvar r)) ->
+               Gamma |- e1 \in T ->
+               Gamma |- (tcasep e e1) \in T
+  | T_CaseB :  forall Gamma e e1 e2 T,
+               Gamma |- e \in TBool ->
+               Gamma |- e1 \in T ->
+               Gamma |- e2 \in T ->
+               Gamma |- (tcaseb e e1 e2) \in T
+  | T_Fail :   forall Gamma T,
+               Gamma |- tfailure \in T
+  | T_Any :    forall Gamma T,
+               Gamma |- T \in_data ->
+               Gamma |- tanything \in T
   
-where "'|-' t '\in' T" := (has_type t T).
+where "Gamma '|-' t '\in' T" := (has_type Gamma t T).
+
+
+
+Example t1 : empty |- ttrue \in TBool.
+Proof. apply T_True. Qed.
+
+Definition con (i : id) := 
+  match i with
+    | (Id 5) => (Some TNat)
+    | _ => None
+end.
+Example t2 : con |- (tvar (Id 5)) \in TNat.
+Proof. apply T_Var. reflexivity. Qed.
+
+Example t3 : con |- (tlet (tvar (Id 5)) tzero (tadd (tsucc tzero) (tvar (Id 5)))) \in TNat.
+Proof. apply T_Let with (T1:=TNat).
+  apply T_Zero.
+  reflexivity.
+  apply T_Add.
+  apply T_Succ. apply T_Zero.
+  apply T_Var. reflexivity.
+Qed.
+
 
 (* anything -> Data type rules? *)
